theories/Spilling/RegLive.v
@@ -10,8 +10,8 @@ Set Implicit Arguments.
 (** * Register Liveness *)
 
 Fixpoint reg_live 
-         (Lv : list ⦃var⦄)
          (ZL : list params)
+         (Lv : list ⦃var⦄)
          (G : ⦃var⦄)
          (s : stmt)
          (sl : spilling)
@@ -20,7 +20,7 @@ Fixpoint reg_live
   :=
     match s, sl with
     | stmtLet x e s, ann1 (Sp, L, _) sl'
-      => let lv_s := reg_live Lv ZL (singleton x) s sl' in
+      => let lv_s := reg_live ZL Lv (singleton x) s sl' in
         (* subtracting L might lead to unnecessary gaps in the liveness, but this is ok:
            variables are killed from the register directly after their last use *)
         ann1 (G ∪ Sp ∪ (((getAnn lv_s) \ singleton x ∪ Exp.freeVars e) \ L)) lv_s
@@ -29,19 +29,19 @@ Fixpoint reg_live
       => ann0 (G ∪ Sp ∪ (Op.freeVars e \ L))
 
     | stmtIf e s1 s2, ann2 (Sp, L, _) sl1 sl2
-      => let lv1 := reg_live Lv ZL ∅ s1 sl1 in
-        let lv2 := reg_live Lv ZL ∅ s2 sl2 in
+      => let lv1 := reg_live ZL Lv ∅ s1 sl1 in
+        let lv2 := reg_live ZL Lv ∅ s2 sl2 in
         ann2 (G ∪ Sp ∪ ((getAnn lv1 ∪ getAnn lv2 ∪ Op.freeVars e) \ L)) lv1 lv2
 
     | stmtApp f Y, ann0 (Sp, L, (_,Sl)::nil)
       => let blv := nth (counted f) Lv ∅ in
         let Z   := nth (counted f) ZL nil in
-        ann0 (G ∪ Sp ∪ (((list_union (Op.freeVars ⊝ Y) ∩ Sl) ∪ blv \ of_list Z) \ L))
+        ann0 (G ∪ Sp ∪ (((list_union (Op.freeVars ⊝ Y) \ Sl) ∪ blv \ of_list Z) \ L))
 
     | stmtFun F t, annF (Sp, L, rms) sl_F sl_t
-      => let lv_t := reg_live (fst ⊝ rms ++ Lv) (fst ⊝ F ++ ZL) ∅ t sl_t in
-        let lv_F := (fun ps sl_s => reg_live (fst ⊝ rms ++ Lv)
-                                          (fst ⊝ F   ++ ZL)
+      => let lv_t := reg_live (fst ⊝ F ++ ZL) (fst ⊝ rms ++ Lv) ∅ t sl_t in
+        let lv_F := (fun ps sl_s => reg_live (fst ⊝ F   ++ ZL)
+                                          (fst ⊝ rms ++ Lv)
                                           (of_list (fst ps))
                                           (snd ps)
                                            sl_s
@@ -52,4 +52,412 @@ Fixpoint reg_live
     end
 .
 
-                                               
+
+
+Inductive rlive_sound
+  : list params -> list (set var) -> stmt -> spilling -> ann (set var) -> Prop :=
+| RLiveLet ZL Lv x e s Sp L sl lv (al:ann (set var))
+  :  Sp ⊆ lv
+     -> rlive_sound ZL Lv s sl al
+     -> live_exp_sound e (lv ∪ L)
+     -> (getAnn al \ singleton x) ⊆ lv ∪ L
+     -> x ∈ getAnn al
+     -> rlive_sound ZL Lv (stmtLet x e s) (ann1 (Sp,L,nil) sl) (ann1 lv al)
+| RLiveIf Lv ZL e s1 s2 Sp L sl1 sl2 lv al1 al2
+  :  Sp ⊆ lv
+     -> rlive_sound ZL Lv s1 sl1 al1
+     -> rlive_sound ZL Lv s2 sl2 al2
+     -> live_op_sound e (lv ∪ L)
+     -> getAnn al1 ⊆ lv ∪ L
+     -> getAnn al2 ⊆ lv ∪ L
+     -> rlive_sound ZL Lv (stmtIf e s1 s2) (ann2 (Sp,L,nil) sl1 sl2) (ann2 lv al1 al2)
+| RLiveApp ZL Lv l Y Sp L R' M' lv blv Z
+  : Sp ⊆ lv
+    -> get ZL (counted l) Z
+    -> get Lv (counted l) blv
+    -> (blv \ of_list Z) ⊆ lv ∪ L
+    -> (forall n y, get Y n y -> live_op_sound y (lv ∪ M' ∪ L))
+    -> rlive_sound ZL Lv (stmtApp l Y) (ann0 (Sp,L,(R',M')::nil)) (ann0 lv)
+| RLiveReturn ZL Lv e Sp L lv
+  : Sp ⊆ lv
+    -> live_op_sound e (lv ∪ L)
+    -> rlive_sound ZL Lv (stmtReturn e) (ann0 (Sp,L,nil)) (ann0 lv)
+| RLiveFun ZL Lv F t lv Sp L rms sl_F sl_t als alb
+  : Sp ⊆ lv
+    -> rlive_sound (fst ⊝ F ++ ZL) (getAnn ⊝ als ++ Lv) t sl_t alb
+    -> (forall n Zs a sl_s, get F n Zs ->
+                 get als n a ->
+                 get sl_F n sl_s ->
+                 rlive_sound (fst ⊝ F ++ ZL) (getAnn ⊝ als ++ Lv) (snd Zs) sl_s a)
+    -> (forall n Zs a, get F n Zs -> (* do I need this? *)
+                 get als n a ->
+                 (of_list (fst Zs)) ⊆ getAnn a (* don't add L here *)
+                 /\ NoDupA eq (fst Zs))
+    -> getAnn alb ⊆ lv ∪ L
+    -> rlive_sound ZL Lv (stmtFun F t) (annF (Sp,L,rms) sl_F sl_t) (annF lv als alb)
+.
+
+
+Lemma reg_live_G_eq
+      (G : ⦃var⦄)
+      (Lv : list ⦃var⦄)
+      (ZL : list params)
+      (s : stmt)
+      (sl : spilling)
+  :
+    getAnn (reg_live ZL Lv G s sl)
+           [=]
+           getAnn (reg_live ZL Lv ∅ s sl) ∪ G
+.
+Proof.
+  general induction s;
+    destruct sl;
+    try destruct a;
+    try destruct p;
+    simpl; eauto; try cset_tac.
+  induction l0; simpl; eauto.
+  - cset_tac.
+  - destruct a. destruct l0; simpl; cset_tac. 
+Qed.
+
+
+
+(* remove ? 
+Lemma reconstr_live_remove_G
+      Lv ZL G s sl G'
+  :
+    getAnn (reconstr_live Lv ZL G s sl) \ G
+           ⊆ getAnn (reconstr_live Lv ZL G' s sl)
+.
+Proof.
+  destruct s, sl, a; simpl; cset_tac.
+Qed.
+*)
+
+
+
+Lemma reg_live_G
+      (Lv : list (set var))
+      (ZL : list (params))
+      (G : set var)
+      (s : stmt)
+      (sl : spilling)
+  :
+    G ⊆ getAnn (reg_live ZL Lv G s sl)
+.
+Proof.
+  induction s,sl; destruct a,p;
+    simpl; eauto with cset.
+  - simpl. induction l0; simpl; eauto with cset.
+    destruct a,l0; simpl; cset_tac.
+Qed.
+
+Require Import Subterm.
+
+Inductive subAnno (X:Type) : ann X -> ann X -> Prop :=
+    subAnno_refl (a : ann X) : subAnno a a
+  | subAnno1 (a b : ann X) (x : X) :
+      subAnno a b -> subAnno a (ann1 x b)
+  | subAnno21 (a b b' : ann X) (x : X) :
+      subAnno a b -> subAnno a (ann2 x b b')
+  | subAnno22 (a b b' : ann X) (x : X) :
+      subAnno a b'-> subAnno a (ann2 x b b')
+  | subAnnoF1 (a b : ann X) (bF : list (ann X)) (x : X) :
+      subAnno a b -> subAnno a (annF x bF b)
+  | subAnnoF2 (a b b' : ann X) (bF : list (ann X)) (x : X) (n : nat) :
+      get bF n b' -> subAnno a b' -> subAnno a (annF x bF b)
+.
+
+
+
+Lemma reg_live_sound k ZL Λ rlv (R M : ⦃var⦄) G s sl
+  : spill_sound k ZL Λ (R,M) s sl
+    -> (forall s' sl',
+          subTerm s' s
+          -> subAnno sl' sl
+          -> match s',sl' with
+            | stmtFun F t, annF (_,rms) sl_F _ =>
+              forall Zs sl_s rm' n, get rlv n rm'
+                              -> get F n Zs
+                              -> get sl_F n sl_s
+                              -> rm' = getAnn (reg_live ZL rlv ∅ (snd Zs) sl_s)
+            | _,_ => True
+            end)
+    -> PIR2 Subset rlv (fst ⊝ Λ) 
+    -> rlive_sound ZL rlv s sl (reg_live ZL rlv G s sl)
+.
+Proof.
+  intros spillSnd inR.
+  general induction spillSnd.
+  - econstructor.
+    + apply union_incl_left; clear;cset_tac.
+    + eapply IHspillSnd; eauto.
+      intros; apply inR; econstructor; eauto.
+    + apply live_exp_sound_incl with (lv':=Exp.freeVars e).
+      * apply live_freeVars.
+      * setoid_rewrite <-incl_right at 4. clear;cset_tac.
+    + setoid_rewrite <-incl_right at 3. clear; cset_tac.
+    + apply reg_live_G. clear; cset_tac.
+  - econstructor.
+    + clear; cset_tac.
+    + apply live_op_sound_incl with (lv':=Op.freeVars e).
+      * apply Op.live_freeVars.
+      * clear; cset_tac.
+  - econstructor.
+    + setoid_rewrite <-incl_right at 3. clear; cset_tac.
+    + eapply IHspillSnd1; eauto.
+      intros; apply inR; econstructor; eauto.
+    + eapply IHspillSnd2; eauto.
+      intros; apply inR; econstructor 4; eauto.
+    + apply live_op_sound_incl with (lv':=Op.freeVars e).
+      * apply Op.live_freeVars.
+      * setoid_rewrite <-incl_right at 4. clear; cset_tac.
+    + setoid_rewrite <-incl_right at 2. clear; cset_tac.
+    + setoid_rewrite <-incl_right at 2. clear; cset_tac.
+  - assert (H8' := H8). eapply PIR2_flip in H8'. eapply PIR2_nth in H8'.
+    destruct H8', H9.
+    econstructor; eauto.
+    + clear; cset_tac.
+    + simpl. erewrite !get_nth; eauto. clear; cset_tac.
+    + intros. inv_get.
+      apply live_op_sound_incl with (lv':=Op.freeVars y).
+      * apply Op.live_freeVars.
+      * erewrite !get_nth; eauto. 
+        erewrite <-incl_list_union with (s:=Op.freeVars y); eauto; clear; cset_tac.
+    + eauto.
+  - econstructor.
+    + setoid_rewrite <-incl_right at 3. clear; cset_tac.
+    + admit.
+    + intros; inv_get. admit.
+    + intros; inv_get. split. admit. (* THIS will most likely need another invariant *) admit.
+    + clear; cset_tac.
+
+      
+    
+11:00 - 17:00 + 18:00 -
+      
+############################################################################################
+############################################################################################
+PROOF of reconstrlv:########################################################################
+############################################################################################
+############################################################################################
+
+  - rewrite do_spill_empty by apply count_clear_zero.
+    unfold do_spill_rec.
+    rewrite do_spill_rm_empty by apply count_clear_zero.
+    simpl.
+    eapply get_get_eq in H; eauto.
+    subst Z0.
+
+    econstructor; eauto.
+    + eapply zip_get; eauto.
+    + simpl.
+      unfold slot_merge.
+      eapply map_get_eq; eauto.
+    + simpl.
+      assert (nth (labN l) (slot_merge slot Λ) ∅ [=] R_f ∪ map slot M_f)
+        as nth_EQ.
+      {
+        unfold slot_merge.
+        assert ((fun RM => fst RM ∪ map slot (snd RM)) (R_f,M_f) = R_f ∪ map slot M_f)
+          by (simpl; reflexivity).
+        eapply map_get_eq in H13; eauto.
+        erewrite get_nth; eauto.
+        reflexivity.
+      }
+      rewrite nth_EQ.
+      assert (of_list (nth (labN l) (slot_lift_params slot ⊜ Λ ZL) nil)
+              [=] of_list (slot_lift_params slot (R_f,M_f) Z))
+        as nth_slp by (erewrite nth_zip; eauto; simpl; reflexivity).
+      rewrite nth_slp.
+      clear; cset_tac.
+    + unfold compute_ib.
+      erewrite nth_zip; eauto.
+      apply sla_extargs_slp_length; eauto.
+    + intros; inv_get.
+      erewrite nth_zip; eauto.
+      erewrite nth_zip in H; eauto.
+      assert (get_x := H).
+      eapply get_Y_from_extargs in get_x as [n' get_x].
+      exploit H5 as is_var; eauto.
+      invc is_var.
+      apply live_op_sound_incl
+      with (lv':= match slot_lift_args slot M' (Var v) with
+                  | Var v => singleton v
+                  | _ => ∅
+                  end
+           );
+        unfold slot_lift_args;
+        simpl.
+      * decide (v ∈ M');
+          econstructor;
+          eauto with cset.
+      * repeat apply incl_union_left.
+        decide (v ∈ M');
+          unfold slot_lift_args;
+          simpl;
+          [ change (singleton (slot v)) with (Op.freeVars (Var (slot v)))
+          | change (singleton v) with (Op.freeVars (Var v)) ];
+          eapply get_list_union_map; eauto;
+          eapply map_get_eq; eauto;
+          simpl;
+          decide (v ∈ M'); simpl; eauto.
+  - rewrite do_spill_empty by apply count_clear_zero.
+    unfold do_spill_rec.
+    rewrite do_spill_rm_empty by apply count_clear_zero.
+    simpl.
+
+    econstructor; simpl; eauto.
+    + apply live_op_sound_incl with (lv':=Op.freeVars e).
+      * apply Op.live_freeVars.
+      * clear; cset_tac.
+
+  - rewrite do_spill_empty by apply count_clear_zero.
+    unfold do_spill_rec.
+    rewrite do_spill_rm_empty by apply count_clear_zero.
+    simpl.
+
+    apply renamedApart_incl in renAp as [renaF rena2].
+    rewrite fst_zip_pair by eauto with len.
+    econstructor; simpl; eauto.
+    + rewrite fst_zip_pair by eauto with len.
+      rewrite slot_merge_app.
+      rewrite slot_lift_params_app; eauto with len.
+
+      apply live_sound_monotone with (LV:= slot_merge slot (rms ++ Λ)).
+      * rewrite <- zip_app.
+        eapply IHlvSnd with (ra:=ant) (R:=R\K ∪ L) (M:=Sp ∪ M); eauto.
+        -- eapply R'_VD with (R:=R) (M:=M); eauto.
+        -- eapply M'_VD with (R:=R) (M:=M); eauto.
+        -- rewrite rena2; eauto.
+        -- eapply getAnn_als_EQ_merge_rms; eauto.
+        -- eapply get_ofl_VD; eauto.
+        -- eauto with len.
+      * rewrite <- slot_merge_app.
+        apply PIR2_app with (L2:=slot_merge slot Λ);
+          swap 1 2.
+        {
+          apply PIR2_refl; eauto.
+        }
+        apply PIR2_get.
+        -- rewrite <- zip_app.
+           intros n x x' H4 H5.
+           unfold slot_merge in H5.
+           inv_get; simpl.
+           rename x into Zs.
+           rename x0 into rm.
+           rename x4 into sl_s.
+           rename x1 into a.
+           rename x2 into al.
+           rename H32 into get_al.
+           rename H31 into get_a.
+           rename H26 into get_sls.
+           rename H29 into get_Zs.
+           rename H5 into get_rm.
+
+           rewrite slot_merge_app.
+
+           exploit H19 as H24'; eauto. (*H31*)
+           exploit H23 as H20'; eauto. (*H32*)
+           exploit renaF as renaF'; eauto.
+           exploit H14 as H15'; eauto. (*H33*)
+           exploit H2 as H2'; eauto.
+           destruct H2' as [H2' _].
+           destruct H15' as [A [B [C E]]].
+           assert (rm = (fst rm, snd rm)) as rm_eta by apply pair_eta.
+           rewrite rm_eta in H24'.
+           erewrite reconstr_live_small with (VD:=VD)
+                                             (ra:=a)
+                                             (R:=fst rm)
+                                             (M:=snd rm); eauto.
+           ++ (*clear - pir2_EQ pir3 renaF H24 H20 H15 H2 H16 H20 H8 H13 H14 H H9 H18 ra_VD.*)
+             clear - rm_eta H2' get_al get_a get_sls get_rm get_Zs H15.
+             rewrite rm_eta in get_rm.
+             eapply al_sub_RfMf in get_rm; eauto.
+             rewrite rm_eta.
+              repeat apply union_incl_split;
+                [clear; cset_tac | clear; cset_tac
+                 | eapply ofl_slp_sub_rm; eauto ].
+           ++ rewrite renaF'; eauto.
+           ++ eapply getAnn_als_EQ_merge_rms; eauto.
+           ++ eapply get_ofl_VD; eauto.
+           ++ eauto with len.
+
+        -- rewrite <- zip_app.
+           rewrite map_length.
+           ++ rewrite zip_length2.
+              ** rewrite zip_length2; eauto with len.
+              ** rewrite zip_length2, map_length;
+                   eauto with len.
+           ++ eauto with len.
+    + symmetry.
+      apply zip_length2.
+      repeat rewrite length_map.
+      rewrite zip_length2;
+        eauto with len.
+    + intros; inv_get.
+      simpl.
+      rewrite fst_zip_pair by eauto with len.
+      rewrite slot_merge_app.
+      rewrite slot_lift_params_app; eauto with len.
+
+      apply live_sound_monotone with (LV:= slot_merge slot (rms ++ Λ)).
+      * rewrite <- zip_app; eauto with len.
+        assert ((fst x2, snd x2) = x2)
+          by (destruct x2; simpl; reflexivity).
+        rewrite <- H4 in H30.
+        exploit H23; eauto.
+        eapply H1 with (ra:=x0) (R:=fst x2) (M:=snd x2); eauto.
+        -- exploit renaF as renaF'; eauto.
+           rewrite renaF'; eauto.
+        -- eapply getAnn_als_EQ_merge_rms; eauto.
+        -- eapply get_ofl_VD; eauto.
+      * rewrite <- slot_merge_app.
+        apply PIR2_app with (L2:=slot_merge slot Λ);
+          swap 1 2.
+        {
+          apply PIR2_refl; eauto.
+        }
+        apply PIR2_get.
+        -- intros.
+           unfold slot_merge in H5.
+           inv_get; simpl.
+           rewrite slot_merge_app.
+           rewrite <- zip_app; eauto with len.
+           exploit H19; eauto.
+           exploit H23; eauto.
+           exploit H9; eauto.
+           destruct x5 as [R_f M_f].
+           erewrite reconstr_live_small with (ra:=x6)
+                                             (VD:=VD)
+                                             (R:=R_f)
+                                             (M:=M_f); eauto.
+           ++ exploit H2 as H2'; eauto; dcr; simpl in *.
+
+             rewrite ofl_slp_sub_rm; eauto. simpl.
+             clear; cset_tac.
+             eapply al_sub_RfMf; eauto.
+           ++ rewrite renaF; eauto.
+           ++ eapply getAnn_als_EQ_merge_rms; eauto.
+           ++ eapply get_ofl_VD; eauto.
+        -- unfold slot_merge. eauto with len.
+    + intros.
+      inv_get.
+      simpl.
+      split; [ | auto].
+      * apply reconstr_live_G.
+      * split; eauto.
+        -- exploit H2; eauto; dcr.
+           eapply PIR2_nth in H15; eauto; dcr.
+           destruct x2. eapply NoDupA_slot_lift_params; eauto.
+           unfold merge in H33.
+           exploit H23; eauto; dcr. eauto with cset.
+           rewrite <- M_VD. unfold union_fs. simpl.
+           rewrite <- H27.
+           rewrite <- incl_list_union; eauto using zip_get; [|reflexivity].
+           unfold defVars. clear; cset_tac.
+Qed.
+        
+
+
+      
