theories/Spilling/SpillMinKill.v
@@ -1,0 +1,112 @@
+Require Import List Map Env AllInRel Exp MoreList.
+Require Import IL Annotation.
+Require Import Liveness.Liveness.
+Require Import ExpVarsBounded SpillSound OneOrEmpty.
+Require Import Take TakeSet.
+
+
+Set Implicit Arguments.
+
+
+(* TODO : - adjust spill_min_kill such that no explicit kill set is necessary 
+          - prove spill_sound -> spill_min_kill *)
+
+
+Inductive spill_min_kill (k:nat) :
+  (list params)
+  -> (list (⦃var⦄ * ⦃var⦄))
+  -> (⦃var⦄ * ⦃var⦄)
+  -> stmt
+  -> spilling
+  -> Prop
+  :=
+
+  | SpillLet
+      (ZL : list params)
+      (Λ : list (⦃var⦄ * ⦃var⦄))
+      (R M Sp L K Kx : ⦃var⦄)
+      (x : var)
+      (e : exp)
+      (s : stmt)
+      (sl : spilling)
+    : Sp ⊆ R
+      -> L ⊆ Sp ∪ M
+      -> spill_min_kill k ZL Λ ({x;(R\K ∪ L)\Kx }, Sp ∪ M) s sl
+      -> Exp.freeVars e ⊆ R\K ∪ L
+      -> k > 0
+      -> cardinal (R\K ∪ L) <= k
+      -> cardinal ({x;((R\K) ∪ L)\Kx }) <= k
+      -> spill_min_kill k ZL Λ (R,M) (stmtLet x e s) (ann1 (Sp,L,nil) sl)
+
+  | SpillReturn
+      (ZL : list (params))
+      (Λ : list (⦃var⦄ * ⦃var⦄))
+      (R M Sp L K : ⦃var⦄)
+      (e : op)
+    : Sp ⊆ R
+      -> L ⊆ Sp ∪ M
+      -> Op.freeVars e ⊆ R\K ∪ L
+      -> cardinal ((R\K) ∪ L) <= k
+      -> spill_min_kill k ZL Λ (R,M) (stmtReturn e)
+                    (ann0 (Sp,L,nil))
+
+  | SpillIf
+      (ZL : list (params))
+      (Λ : list (⦃var⦄ * ⦃var⦄))
+      (R M Sp L K : ⦃var⦄)
+      (e : op)
+      (s t : stmt)
+      (sl_s sl_t : spilling)
+
+    : Sp ⊆ R
+      -> L ⊆ Sp ∪ M
+      -> Op.freeVars e ⊆ R\K ∪ L
+      -> cardinal (R\K ∪ L) <= k
+      -> spill_min_kill k ZL Λ (R\K ∪ L, Sp ∪ M) s sl_s
+      -> spill_min_kill k ZL Λ (R\K ∪ L, Sp ∪ M) t sl_t
+      -> spill_min_kill k ZL Λ (R,M) (stmtIf e s t) (ann2 (Sp,L,nil) sl_s sl_t)
+
+  | SpillApp
+      (ZL : list params)
+      (Λ : list (⦃var⦄ * ⦃var⦄))
+      (R M Sp L K R_f M_f R' M' : ⦃var⦄)
+      (f : lab)
+      (Z : params)
+      (Y : args)
+    : Sp ⊆ R
+      -> L ⊆ Sp ∪ M
+      -> cardinal (R\K ∪ L) <= k
+      -> get ZL (counted f) Z
+      -> get Λ (counted f) (R_f,M_f)
+      -> R_f \ of_list Z ⊆ R\K ∪ L
+      -> M_f \ of_list Z ⊆ Sp ∪ M
+      -> list_union (Op.freeVars ⊝ Y) ⊆ (R\K ∪ L) ∪ M'
+      -> M' ⊆ Sp ∪ M
+      -> spill_min_kill k ZL Λ (R,M) (stmtApp f Y)
+                       (ann0 (Sp,L, (R', M')::nil))
+
+  | SpillFun
+      (ZL : list params)
+      (Λ rms : list (⦃var⦄ * ⦃var⦄))
+      (R M Sp L K : ⦃var⦄)
+      (F : list (params * stmt))
+      (t : stmt)
+      (sl_F : list spilling)
+      (sl_t : spilling)
+    : Sp ⊆ R
+      -> L ⊆ Sp ∪ M
+      -> cardinal (R\K ∪ L) <= k
+      -> length F = length sl_F
+      -> length F = length rms
+      -> (forall n rm, get rms n rm -> cardinal (fst rm) <= k)
+      -> (forall n Zs rm sl_s, get rms n rm
+                         -> get F n Zs
+                         -> get sl_F n sl_s
+                         -> spill_min_kill k ((fst ⊝ F) ++ ZL)
+                                          (rms ++ Λ) rm (snd Zs) sl_s
+        )
+      -> spill_min_kill k ((fst ⊝ F) ++ ZL) (rms ++ Λ) (R\K ∪ L, Sp ∪ M) t sl_t
+      -> spill_min_kill k ZL Λ (R,M) (stmtFun F t)
+                       (annF (Sp,L,rms) sl_F sl_t)
+.
+
